completed gradual_rec.v

proofs/itrees/gradual_rec.v
@@ -2,304 +2,161 @@
 From ExtLib Require Import
      Structures.Monad.
 
+From Coq Require Import
+     Setoid
+     Morphisms.
+
 From ITree Require Import
-     Basics.Utils
-     Axioms
+     Basics.Utils 
      ITree
      Eq
-     Basics.
-
+     Basics
+     Core.ITreeDefinition
+     Core.KTree
+     Core.KTreeFacts
+     Indexed.Sum
+     Indexed.Function
+     Indexed.Relation
+     RecursionFacts
+     InterpFacts.
+     
 From Paco Require Import paco.
 
 Require Import List.
+
+Require Import it_sems_core.
 
 Import Monads.
 Import MonadNotation.
 Local Open Scope monad_scope.
 
-
-(** Type function isomorphism class *)
-Class FIso (E1 E2: Type -> Type) : Type := FI {
-    mfun1: E1 -< E2 ;
-    mfun2: E2 -< E1 ; 
-    mid12 : forall (T: Type) x, @mfun1 T (@mfun2 T x) = x ; 
-    mid21 : forall (T: Type) x, @mfun2 T (@mfun1 T x) = x ;
-}.
-
-Lemma FIsoRev {E1 E2} (X: FIso E1 E2) : FIso E2 E1.
-destruct X.
-econstructor; auto.
-Defined.
-
-Lemma FIsoId E : FIso E E.
-econstructor; auto.
-Defined.
-
-Global Instance FIsoTrans {E1 E2 E3} (X: FIso E1 E2) (Y: FIso E2 E3) :
-  FIso E1 E3.
-destruct X.
-destruct Y.
-set (mf1 := fun X x => mfun5 X (mfun3 X x)).
-set (mf2 := fun X x => mfun4 X (mfun6 X x)).
-econstructor; eauto; intros.
-- instantiate (1:= mf2).
-  instantiate (1:= mf1).
-  subst mf1 mf2; simpl; intros; auto.
-  rewrite mid13.
-  rewrite mid14; auto. 
-- subst mf1 mf2; simpl; auto.
-  rewrite mid23.
-  rewrite mid22; auto.
-Defined.  
-  
-Global Instance FIsoSum {E1 E2 E3 E4} (X: FIso E1 E2) (Y: FIso E3 E4) :
-  FIso (E1 +' E3) (E2 +' E4).
-destruct X.
-destruct Y.
-econstructor;
-  unfold ReSum_sum, case_, Case_sum1, case_sum1, resum, ReSum_inl,
-    ReSum_inr, cat, Cat_IFun, inl_, inr_, Inl_sum1, Inr_sum1, resum;
-  simpl; intros.
-- destruct x.
-  + rewrite mid13; auto.
-  + rewrite mid14; auto.
-- destruct x.
-  + rewrite mid22; auto.
-  + rewrite mid23; auto.
-Defined.
-
-Lemma FIsoIdL E : FIso E (E +' void1).
-econstructor;
-  unfold ReSum_sum, case_, Case_sum1, case_sum1, resum, ReSum_inl,
-    ReSum_inr, cat, Cat_IFun, inl_, inr_, Inl_sum1, Inr_sum1, resum,
-    ReSum_id, id_, Id_IFun; 
-  simpl; intros; auto.
-destruct x; auto.
-destruct v.
-Defined.
-
-Lemma FIsoIdR E : FIso E (void1 +' E).
-econstructor;
-  unfold ReSum_sum, case_, Case_sum1, case_sum1, resum, ReSum_inl,
-    ReSum_inr, cat, Cat_IFun, inl_, inr_, Inl_sum1, Inr_sum1, resum,
-    ReSum_id, id_, Id_IFun; 
-  simpl; intros; auto.
-destruct x; auto.
-destruct v.
-Defined.
-
-Lemma FIsoRAssoc E1 E2 E3 :
-  FIso ((E1 +' E2) +' E3) (E1 +' (E2 +' E3)).
-econstructor;
-  unfold ReSum_sum, case_, Case_sum1, case_sum1, resum, ReSum_inl,
-    ReSum_inr, cat, Cat_IFun, inl_, inr_, Inl_sum1, Inr_sum1, resum,
-    ReSum_id, id_, Id_IFun;
-  simpl; intros; auto; destruct x; auto; destruct s; auto.
-Defined.
-
-Lemma FIsoLAssoc E1 E2 E3 :
-  FIso (E1 +' (E2 +' E3)) ((E1 +' E2) +' E3).
-econstructor;
-  unfold ReSum_sum, case_, Case_sum1, case_sum1, resum, ReSum_inl,
-    ReSum_inr, cat, Cat_IFun, inl_, inr_, Inl_sum1, Inr_sum1, resum,
-    ReSum_id, id_, Id_IFun;
-  simpl; intros; auto; destruct x; auto; destruct s; auto.
-Defined.
-
-Lemma FIsoComm E1 E2 : FIso (E1 +' E2) (E2 +' E1).
-econstructor;
-  unfold ReSum_sum, case_, Case_sum1, case_sum1, resum, ReSum_inl,
-    ReSum_inr, cat, Cat_IFun, inl_, inr_, Inl_sum1, Inr_sum1, resum,
-    ReSum_id, id_, Id_IFun;
-  simpl; intros; auto; destruct x; auto. 
-Defined.
-
-
-(** instances for mutual recursion *)
-
-Definition FIso_MR Em {E1 E0 Er} (X: FIso E1 (E0 +' Er)) :
-  FIso (Em +' E1) ((Em +' E0) +' Er) :=
-  FIsoTrans (FIsoSum (FIsoId Em) X) (FIsoLAssoc Em E0 Er).  
-
-
-Lemma FIso_MR_proj11' Em {E1 E0 Er} (X: FIso E1 (E0 +' Er)) :
-  let Y:= FIso_MR Em X in 
-  forall A (e: Em A), mfun1 (inl1 e) = inl1 (inl1 e).
-Proof.
-  simpl; intros.
-  destruct X.
-  unfold mfun1; simpl.
-  unfold ReSum_sum, case_, Case_sum1, case_sum1, resum, ReSum_inl,
-    ReSum_inr, cat, Cat_IFun, inl_, inr_, Inl_sum1, Inr_sum1, resum,
-    ReSum_id, id_, Id_IFun; auto.
-Qed.
-  
-Lemma FIso_MR_proj11 Em {E1 E0 Er} (X: FIso E1 (E0 +' Er)) Y :
-  Y = FIso_MR Em X ->  
-  forall A (e: Em A), mfun1 (inl1 e) = inl1 (inl1 e).
-Proof.
-  simpl; intros.
-  inv H; eapply FIso_MR_proj11'. 
-Qed.
-
-Lemma FIso_MR_proj12' Em {E1 E0 Er} (X: FIso E1 (E0 +' Er)) :
-  let Y:= FIso_MR Em X in 
-  forall A (e: E1 A), @mfun1 _ _ Y A (inr1 e) = 
-                        match (@mfun1 _ _ X A e) with
-                        | inl1 x => inl1 (inr1 x)
-                        | inr1 x => inr1 x end.                 
-Proof.
-  simpl; intros.
-  destruct X.
-  unfold mfun1; simpl.
-  unfold ReSum_sum, case_, Case_sum1, case_sum1, resum, ReSum_inl,
-    ReSum_inr, cat, Cat_IFun, inl_, inr_, Inl_sum1, Inr_sum1, resum,
-    ReSum_id, id_, Id_IFun; auto.
-Qed.
-  
-Lemma FIso_MR_proj12 Em {E1 E0 Er} (X: FIso E1 (E0 +' Er)) Y :
-  Y = FIso_MR Em X -> 
-  forall A (e: E1 A), @mfun1 _ _ Y A (inr1 e) = 
-                        match (@mfun1 _ _ X A e) with
-                        | inl1 x => inl1 (inr1 x)
-                        | inr1 x => inr1 x end.                 
-Proof.
-  simpl; intros.
-  inv H; eapply FIso_MR_proj12'. 
-Qed.
-  
-Lemma FIso_MR_proj1' E1 {E2 E3 E4} (X: FIso E2 (E3 +' E4)) : 
-  let Y:= FIso_MR E1 X in
-  forall A (e: E1 A), mfun2 (inl1 (inl1 e)) = inl1 e.
-Proof.  
-  simpl; intros.
-  destruct X.
-  unfold mfun2; simpl.
-  unfold ReSum_sum, case_, Case_sum1, case_sum1, resum, ReSum_inl,
-    ReSum_inr, cat, Cat_IFun, inl_, inr_, Inl_sum1, Inr_sum1, resum,
-    ReSum_id, id_, Id_IFun; auto.
-Qed.
-
-Lemma FIso_MR_proj1 E1 {E2 E3 E4} (X: FIso E2 (E3 +' E4)) Y : 
-  Y = FIso_MR E1 X ->
-  forall A (e: E1 A), mfun2 (inl1 (inl1 e)) = inl1 e.
-Proof.  
-  simpl; intros.
-  inv H; eapply FIso_MR_proj1'. 
-Qed.
-
-Lemma FIso_MR_proj3' E1 {E2 E3 E4} (X: FIso E2 (E3 +' E4)) : 
-  let Y:= @FIso_MR E1 E2 E3 E4 X in
-  forall A (e: E3 A), mfun2 (inl1 (inr1 e)) =
-                        inr1 (@mfun2 E2 (E3 +' E4) X _ (inl1 e)).
-Proof.  
-  simpl; intros.
-  destruct X.
-  unfold mfun2, mfun1; simpl.
-  unfold ReSum_sum, case_, Case_sum1, case_sum1, resum, ReSum_inl,
-    ReSum_inr, cat, Cat_IFun, inl_, inr_, Inl_sum1, Inr_sum1, resum,
-    ReSum_id, id_, Id_IFun; auto.
-Qed.
-
-Lemma FIso_MR_proj3 E1 {E2 E3 E4} (X: FIso E2 (E3 +' E4)) Y : 
-  Y = FIso_MR E1 X ->
-  forall A (e: E3 A), mfun2 (inl1 (inr1 e)) = inr1 (mfun2 (inl1 e)).
-Proof.  
-  simpl; intros.
-  inv H; eapply FIso_MR_proj3'. 
-Qed.
-
-Lemma FIso_MR_proj4' E1 {E2 E3 E4} (X: FIso E2 (E3 +' E4)) : 
-  let Y:= FIso_MR E1 X in
-  forall A (e: E4 A), mfun2 (inr1 e) = inr1 (mfun2 (inr1 e)).
-Proof.  
-  simpl; intros.
-  destruct X.
-  unfold mfun2, mfun1; simpl.
-  unfold ReSum_sum, case_, Case_sum1, case_sum1, resum, ReSum_inl,
-    ReSum_inr, cat, Cat_IFun, inl_, inr_, Inl_sum1, Inr_sum1, resum,
-    ReSum_id, id_, Id_IFun; auto.
-Qed.
-
-Lemma FIso_MR_proj4 E1 {E2 E3 E4} (X: FIso E2 (E3 +' E4)) Y : 
-  Y = FIso_MR E1 X ->
-  forall A (e: E4 A), mfun2 (inr1 e) = inr1 (mfun2 (inr1 e)).
-Proof.  
-  simpl; intros.
-  inv H; eapply FIso_MR_proj4'. 
-Qed.
-
-(***************************************************************************)
-
-(* begin hide *)
-From ITree Require Import
-     Basics.Basics
-     Basics.Category
-     Core.ITreeDefinition
-     Indexed.Sum
-     Interp.Interp
-     Indexed.Relation
-     Core.Subevent.
-
 Import ITreeNotations.
 #[local] Open Scope itree_scope.
-(* end hide *)
 
-Definition ext_handler {D1 E : Type -> Type} 
-  (ctx : D1 ~> itree E) : (D1 +' E) ~> itree E :=
-  fun X e => match e with
-             | inl1 e' => ctx _ e'
-             | inr1 e' => trigger e' end.                 
+(** event-based recursion to support inlining, by splitting and
+    gradualizing. largely based on ITree.Recursion and
+    ITree.RecursionFacts. *)
 
-(** two alternative ways **)
+(* auxiliary lemma *)
+Lemma FIsoSum {E1 E2 E3 E4} (X: FIso E1 E2) (Y: FIso E3 E4) :
+  FIso (E1 +' E3) (E2 +' E4).
+Proof.  
+  set (mf1 := fun T (x: (E1 +' E3) T) => match x with
+                          | inl1 x' => inl1 (@mfun1 _ _ X _ x')
+                          | inr1 x' => inr1 (@mfun1 _ _ Y _ x') end).
+  set (mf2 := fun T (x: (E2 +' E4) T) => match x with
+                          | inl1 x' => inl1 (@mfun2 _ _ X _ x')
+                          | inr1 x' => inr1 (@mfun2 _ _ Y _ x') end).
+  econstructor 1 with (mfun1 := mf1) (mfun2 := mf2).
+  - intros T [x | x]; simpl; rewrite mid12; auto.
+  - intros T [x | x]; simpl; rewrite mid21; auto.
+Qed.    
 
-(** plan A (probably better) *)
+(* version of interp_mrec that splits recursion events into two *)
+Definition interp_mrec2 {D1 D2 D E : Type -> Type}
+   (X: FIso D (D1 +' D2))
+   (ctx1 : D1 ~> itree (D +' E))
+   (ctx2 : D2 ~> itree (D +' E)) : itree (D +' E) ~> itree E :=
+  fun R =>
+    ITree.iter (fun t : itree (D +' E) R =>
+      match observe t with
+      | RetF r => Ret (inr r)
+      | TauF t => Ret (inl t)
+      | VisF _ (inl1 d) k => match mfun1 d with
+                           | inl1 d1 => Ret (inl (ctx1 _ d1 >>= k))  
+                           | inr1 d2 => Ret (inl (ctx2 _ d2 >>= k))  
+                           end 
+      | VisF _ (inr1 e) k => Vis e (fun x => Ret (inl (k x)))
+      end).
 
-Definition ext_rassoc_handler {D1 D2 D E : Type -> Type}
-  (X: FIso D (D1 +' D2))
-  (ctx : D1 ~> itree (D2 +' E)) : (D +' E) ~> itree (D2 +' E) :=
-  fun _ e => match e with
-             | inl1 d => match (@mfun1 _ _ X _ d) with
-                         | inl1 d1 => ctx _ d1
-                         | inr1 d2 => trigger d2
-                         end                      
-             | inr1 e' => trigger e' end.                 
-
-Definition rassoc_interpA {D1 D2 D E : Type -> Type}
-  (X: FIso D (D1 +' D2)) (ctx : D1 ~> itree (D2 +' E)) :
-  itree (D +' E) ~> itree (D2 +' E) :=
-  fun _ t1 => interp (@ext_rassoc_handler D1 D2 D E X ctx) t1. 
+(* consistency lemma w.r.t. interp_mrec *)
+Lemma interp_mrec2_ok {D1 D2 D E : Type -> Type}
+   (X: FIso D (D1 +' D2))
+   (ctx1 : D1 ~> itree (D +' E))
+   (ctx2 : D2 ~> itree (D +' E)) R (t1: itree (D +' E) R) :
+  let ctx : D ~> itree (D +' E) :=
+          fun R (e: D R) => match (@mfun1 _ _ X _ e) with
+                            | inl1 e' => ctx1 _ e'
+                            | inr1 e' => ctx2 _ e' end in  
+  eutt eq (interp_mrec ctx t1) (interp_mrec2 X ctx1 ctx2 t1).
+Proof.  
+  unfold interp_mrec2, interp_mrec; simpl.
+  eapply eutt_iter; unfold pointwise_relation.
+  clear t1; intros t1.
+  destruct (observe t1) eqn: ot1; try reflexivity.
+  destruct e; simpl; try reflexivity.
+  destruct (mfun1 d); reflexivity.
+Qed.      
   
-(** plan B *)
+Arguments interp_mrec2 {D1 D2 D E} & X ctx1 ctx2 [T].
 
-Definition rassoc_translate {D1 D2 D E : Type -> Type}
-  (X: FIso D (D1 +' D2)) (T: Type) :
-  itree (D +' E) T -> itree (D1 +' D2 +' E) T :=
-  let X1 := FIsoSum X (FIsoId E) in
-  let X2 := FIsoRAssoc D1 D2 E in
-  let X3 := FIsoTrans X1 X2 in 
-  fun t1 => @translate (D +' E) (D1 +' D2 +' E) (@mfun1 _ _ X3) T t1. 
+(** splitting version of mrec *)
+Definition mrec2 {D1 D2 D E : Type -> Type}
+   (X: FIso D (D1 +' D2))
+   (ctx1 : D1 ~> itree (D +' E))
+   (ctx2 : D2 ~> itree (D +' E)) : D ~> itree E :=
+  let ctx : D ~> itree (D +' E) :=
+          fun R (e: D R) => match (@mfun1 _ _ X _ e) with
+                            | inl1 e' => ctx1 _ e'
+                            | inr1 e' => ctx2 _ e' end in  
+  fun R d => interp_mrec2 X ctx1 ctx2 (ctx _ d).
+  
+Arguments mrec2 {D1 D2 D E} & X ctx1 ctx2 [T].
 
-Definition interp2 {D1 D2 E : Type -> Type} 
-  (ctx : D1 ~> itree (D2 +' E)) :
-  itree (D1 +' D2 +' E) ~> itree (D2 +' E) :=
-  interp (@ext_handler D1 (D2 +' E) ctx).
+Definition trigger_inl1_l {D1 D2 D E : Type -> Type}
+   (X: FIso D (D1 +' D2)) : D1 ~> itree (D +' E) :=
+  fun _ d => ITree.trigger (inl1 (@mfun2 _ _ X _ (inl1 d))).
 
-Definition rassoc_interpB {D1 D2 D E : Type -> Type}
-  (X: FIso D (D1 +' D2)) (ctx : D1 ~> itree (D2 +' E)) :
-  itree (D +' E) ~> itree (D2 +' E) :=
-  fun R t1 => @interp2 D1 D2 E ctx _ (@rassoc_translate D1 D2 D E X R t1). 
+Definition trigger_inl1_r {D1 D2 D E : Type -> Type}
+   (X: FIso D (D1 +' D2)) : D2 ~> itree (D +' E) :=
+  fun _ d => ITree.trigger (inl1 (@mfun2 _ _ X _ (inr1 d))).
 
-(*************)
+Arguments trigger_inl1_l {D1 D2 D E} & X [T].
+Arguments trigger_inl1_r {D1 D2 D E} & X [T].
 
-(* stricter version, with separating handlers *)
-Definition gradual_interp_mrec {D1 D2 D E : Type -> Type} (X: FIso D (D1 +' D2))
-  (ctx1 : D1 ~> itree (D2 +' E)) (ctx2 : D2 ~> itree (D2 +' E)) :
-  itree (D +' E) ~> itree E :=
-  fun R t1 => interp_mrec ctx2 (rassoc_interpA X ctx1 t1).  
+(** Short for endofunctions. *)
+Local Notation endo T := (T -> T).
 
-Definition wk_lassoc_translate {D1 D2 D E : Type -> Type}
-  (X: FIso D (D1 +' D2)) : itree (D2 +' E) ~> itree (D +' E) :=
+Definition mrec2_fix {D1 D2 D E : Type -> Type}
+   (X: FIso D (D1 +' D2))
+   (ctx1 : endo (D1 ~> itree (D +' E)))
+   (ctx2 : endo (D2 ~> itree (D +' E))) : D ~> itree E :=
+  mrec2 X (ctx1 (trigger_inl1_l X)) (ctx2 (trigger_inl1_r X)).
+
+Arguments mrec2_fix {D1 D2 D E} &.
+
+(* splitting version of rec. *)
+Definition rec2 {A1 A2 B: Type} {D E : Type -> Type}
+   (X: FIso D (callE A1 B +' callE A2 B))
+   (body1 : A1 -> itree (D +' E) B)
+   (body2 : A2 -> itree (D +' E) B) : A1 + A2 -> itree E B :=
+  fun a => mrec2 X (calling' body1) (calling' body2) 
+             (match a with
+              | inl a' => @mfun2 _ _ X _ (inl1 (Call a'))
+              | inr a' => @mfun2 _ _ X _ (inr1 (Call a')) end).
+
+Definition call_l {A1 A2 B: Type} {D E : Type -> Type}
+   (X: FIso D (callE A1 B +' callE A2 B)) (a: A1) : itree (D +' E) B :=
+  ITree.trigger (inl1 (@mfun2 _ _ X _ (inl1 (Call a)))).
+
+Definition call_r {A1 A2 B: Type} {D E : Type -> Type}
+   (X: FIso D (callE A1 B +' callE A2 B)) (a: A2) : itree (D +' E) B :=
+  ITree.trigger (inl1 (@mfun2 _ _ X _ (inr1 (Call a)))).
+
+Definition rec2_fix {A1 A2 B: Type} {D E : Type -> Type}
+   (X: FIso D (callE A1 B +' callE A2 B))
+   (body1 : endo (A1 -> itree (D +' E) B))
+   (body2 : endo (A2 -> itree (D +' E) B)) :
+  A1 + A2 -> itree E B := rec2 X (body1 (call_l X)) (body2 (call_r X)).
+
+Arguments rec2_fix {A1 A2 B D E} &.
+
+
+(** gradual recursion *)
+
+(* weakens the itree by extending the events by left associativity *)
+Definition xlassoc_translate {D1 D2 D E : Type -> Type}
+   (X: FIso D (D1 +' D2)) : itree (D2 +' E) ~> itree (D +' E) :=
   let X1 := FIsoSum X (FIsoId E) in
   let f : D2 +' E ~> D +' E :=
       fun _ e => match e with
@@ -307,193 +164,167 @@ Definition wk_lassoc_translate {D1 D2 D E : Type -> Type}
                  | inr1 e' => inr1 e' end in
  fun T t1 => @translate (D2 +' E) (D +' E) (fun _ e => f _ e) T t1.
 
-Definition wk_handler1 {D1 D2 D E : Type -> Type} (X: FIso D (D1 +' D2))
-  (ctx: D1 ~> itree (D2 +' E)) : D1 ~> itree (D +' E) :=
-  fun _ e => wk_lassoc_translate X (ctx _ e).
+Definition wk_handler_l {D1 D2 D E : Type -> Type} (X: FIso D (D1 +' D2))
+   (ctx: D1 ~> itree (D2 +' E)) : D1 ~> itree (D +' E) :=
+  fun _ e => xlassoc_translate X (ctx _ e).
 
-Definition wk_handler2 {D1 D2 D E : Type -> Type} (X: FIso D (D1 +' D2))
-  (ctx: D2 ~> itree (D2 +' E)) : D2 ~> itree (D +' E) :=
-  fun _ e => wk_lassoc_translate X (ctx _ e).
+Definition wk_handler_r {D1 D2 D E : Type -> Type} (X: FIso D (D1 +' D2))
+   (ctx: D2 ~> itree (D2 +' E)) : D2 ~> itree (D +' E) :=
+  fun _ e => xlassoc_translate X (ctx _ e).
 
-(* consistency lemma for the strict version *)
-Lemma gradual_interp_mrec_ok {D1 D2 D E : Type -> Type} (X: FIso D (D1 +' D2))
-  (ctx1 : D1 ~> itree (D2 +' E)) (ctx2 : D2 ~> itree (D2 +' E)) R
-  (t1: itree (D +' E) R) :
-  let ctx01 : D1 ~> itree (D +' E) := wk_handler1 X ctx1 in
-  let ctx02 : D2 ~> itree (D +' E) := wk_handler2 X ctx2 in
+(* splitting recursion into two handlers, where the first one is
+   non-recursive *)
+Definition gradual_interp_mrec {D1 D2 D E : Type -> Type}
+   (X: FIso D (D1 +' D2))
+   (ctx1 : D1 ~> itree (D2 +' E)) (ctx2 : D2 ~> itree (D +' E)) :
+   itree (D +' E) ~> itree E :=
+  fun R t1 =>
+  let ctx01 : D1 ~> itree (D +' E) := wk_handler_l X ctx1 in
+    interp_mrec2 X ctx01 ctx2 t1. 
+
+Arguments gradual_interp_mrec {D1 D2 D E} & X ctx1 ctx2 [T].
+
+(* consistency lemma *)
+Lemma gradual_interp_mrec_ok {D1 D2 D E : Type -> Type}
+   (X: FIso D (D1 +' D2))
+   (ctx1 : D1 ~> itree (D2 +' E)) (ctx2 : D2 ~> itree (D +' E)) R
+   (t1: itree (D +' E) R) :
+  let ctx01 : D1 ~> itree (D +' E) := wk_handler_l X ctx1 in
+  let ctx : D ~> itree (D +' E) :=
+          fun R (e: D R) => match (@mfun1 _ _ X _ e) with
+                            | inl1 e' => ctx01 _ e'
+                            | inr1 e' => ctx2 _ e' end in  
+  eutt eq (interp_mrec ctx t1) (gradual_interp_mrec X ctx1 ctx2 t1).
+Proof.
+  unfold gradual_interp_mrec.
+  eapply interp_mrec2_ok. 
+Qed.
+
+(* stricter version, where additionally the second handler is
+   separating w.r.t. the first *)
+Definition sgradual_interp_mrec {D1 D2 D E : Type -> Type}
+   (X: FIso D (D1 +' D2))
+   (ctx1 : D1 ~> itree (D2 +' E)) (ctx2 : D2 ~> itree (D2 +' E)) :
+   itree (D +' E) ~> itree E :=
+  fun R t1 =>
+  let ctx01 : D1 ~> itree (D +' E) := wk_handler_l X ctx1 in
+  let ctx02 : D2 ~> itree (D +' E) := wk_handler_r X ctx2 in
+    interp_mrec2 X ctx01 ctx02 t1. 
+
+(* consistency lemma *)
+Lemma sgradual_interp_mrec_ok {D1 D2 D E : Type -> Type}
+   (X: FIso D (D1 +' D2))
+   (ctx1 : D1 ~> itree (D2 +' E)) (ctx2 : D2 ~> itree (D2 +' E)) R
+   (t1: itree (D +' E) R) :
+  let ctx01 : D1 ~> itree (D +' E) := wk_handler_l X ctx1 in
+  let ctx02 : D2 ~> itree (D +' E) := wk_handler_r X ctx2 in
   let ctx : D ~> itree (D +' E) :=
           fun R (e: D R) => match (@mfun1 _ _ X _ e) with
                             | inl1 e' => ctx01 _ e'
                             | inr1 e' => ctx02 _ e' end in  
-    eutt eq (interp_mrec ctx t1) (gradual_interp_mrec X ctx1 ctx2 t1). 
-Admitted.  
-
-Definition ext_interp_mrec {D1 D2 D E : Type -> Type}
-  (X: FIso D (D1 +' D2))
-  (ctx1 : D1 ~> itree (D +' E)) (ctx2 : D2 ~> itree (D +' E)) :
-  itree (D +' E) ~> itree E :=
-  fun R =>
-    ITree.iter (fun t : itree (D +' E) R =>
-      match observe t with
-      | RetF r => Ret (inr r)
-      | TauF t => Ret (inl t)
-      | VisF (inl1 d) k => match mfun1 d with
-                           | inl1 d1 => Ret (inl (ctx1 _ d1 >>= k))  
-                           | inr1 d1 => Ret (inl (ctx2 _ d1 >>= k))  
-                           end 
-      | VisF (inr1 e) k => Vis e (fun x => Ret (inl (k x)))
-      end).
-
-(* looser version, non-separating handlers *)
-Definition ext_gradual_interp_mrec {D1 D2 D E : Type -> Type}
-  (X: FIso D (D1 +' D2))
-  (ctx1 : D1 ~> itree (D2 +' E)) (ctx2 : D2 ~> itree (D +' E)) :
-  itree (D +' E) ~> itree E :=
-  fun R t1 =>
-  let ctx01 : D1 ~> itree (D +' E) := wk_handler1 X ctx1 in
-    ext_interp_mrec X ctx01 ctx2 t1. 
-
-(* consistency lemma for the loose version *)
-Lemma ext_gradual_interp_mrec_ok {D1 D2 D E : Type -> Type}
-  (X: FIso D (D1 +' D2))
-  (ctx1 : D1 ~> itree (D2 +' E)) (ctx2 : D2 ~> itree (D +' E)) R
-  (t1: itree (D +' E) R) :
-  let ctx01 : D1 ~> itree (D +' E) := wk_handler1 X ctx1 in
-  let ctx : D ~> itree (D +' E) :=
-          fun R (e: D R) => match (@mfun1 _ _ X _ e) with
-                            | inl1 e' => ctx01 _ e'
-                            | inr1 e' => ctx2 _ e' end in  
-    eutt eq (interp_mrec ctx t1) (ext_gradual_interp_mrec X ctx1 ctx2 t1). 
-Admitted.  
-
-Arguments ext_gradual_interp_mrec {D1 D2 D E} & X ctx1 ctx2 [T].
-
-(** Unfold a mutually recursive definition into separate trees,
-    resolving the mutual references. *)
-Definition ext_gradual_mrec {D1 D2 D E : Type -> Type} (X: FIso D (D1 +' D2))
-  (ctx1 : D1 ~> itree (D2 +' E)) (ctx2 : D2 ~> itree (D +' E))
-  : D ~> itree E :=
-  let ctx01 : D1 ~> itree (D +' E) := wk_handler1 X ctx1 in
-  let ctx : D ~> itree (D +' E) :=
-          fun R (e: D R) => match (@mfun1 _ _ X _ e) with
-                            | inl1 e' => ctx01 _ e'
-                            | inr1 e' => ctx2 _ e' end in  
-  fun R d => ext_gradual_interp_mrec X ctx1 ctx2 (ctx _ d).
+    eutt eq (interp_mrec ctx t1) (sgradual_interp_mrec X ctx1 ctx2 t1). 
+Proof.
+  unfold sgradual_interp_mrec.
+  eapply interp_mrec2_ok. 
+Qed.
   
-Arguments ext_gradual_mrec {D1 D2 D E} & X ctx1 ctx2 [T].
+Arguments sgradual_interp_mrec {D1 D2 D E} & X ctx1 ctx2 [T].
+
+Definition gradual_mrec {D1 D2 D E : Type -> Type}
+   (X: FIso D (D1 +' D2))
+   (ctx1 : D1 ~> itree (D2 +' E))
+   (ctx2 : D2 ~> itree (D +' E)) : D ~> itree E :=
+  let ctx01 : D1 ~> itree (D +' E) := wk_handler_l X ctx1 in
+  mrec2 X ctx01 ctx2. 
+    
+Arguments gradual_mrec {D1 D2 D E} & X ctx1 ctx2 [T].
+
+Definition sgradual_mrec {D1 D2 D E : Type -> Type}
+   (X: FIso D (D1 +' D2))
+   (ctx1 : D1 ~> itree (D2 +' E)) 
+   (ctx2 : D2 ~> itree (D2 +' E)) : D ~> itree E :=
+  let ctx01 : D1 ~> itree (D +' E) := wk_handler_l X ctx1 in
+  let ctx02 : D2 ~> itree (D +' E) := wk_handler_r X ctx2 in
+  mrec2 X ctx01 ctx02. 
+    
+Arguments sgradual_mrec {D1 D2 D E} & X ctx1 ctx2 [T].
 
 
-(***********************************************************************)
+Section Facts.
 
-(* type of an indexed version of interp_mrec. not ideal, seems to
-complicate things too much *)
-(*
-Definition indexed_interp_mrec {I: Type} (P: I -> bool)
-  {D: I -> Type -> Type} {E : Type -> Type}
-  (ctx : (fun X => sigT (fun i => ((P i = true) * D i X)%type)) ~>
-         fun X => sigT (fun i => itree (D i +' E) X)) :
-  (fun X => sigT (fun i => itree (D i +' E) X)) ~>
-    fun X => sigT (fun i => ((P i = false) * itree (D i +' E) X)%type).
-Admitted. 
-*)
+Context {D1 D2 D E : Type -> Type} (X: FIso D (D1 +' D2))
+  (ctx1 : D1 ~> itree (D +' E)) (ctx2 : D2 ~> itree (D +' E)).
 
-(*
-Definition wk_ext_handler {D1 D2 E : Type -> Type}
-  (ctx : D1 ~> itree E) : (D1 +' E) ~> itree (D2 +' E) :=
-  fun X e => match e with
-             | inl1 e' => ctx _ e'
-             | inr1 e' => trigger e' end.                 
-
-Definition ext_interp {D1 D2 E : Type -> Type} {X: D2 -< E}
-  (ctx : D1 ~> itree E) :
-  itree (D1 +' E) ~> itree E :=
-  interp (@ext_handler D1 D2 E X ctx).
-*)
-
-(*
-
-(** Make a recursive call in the handler argument of [mrec]. *)
-Definition trigger_inl1 {D E : Type -> Type} : D ~> itree (D +' E)
-  := fun _ d => ITree.trigger (inl1 d).
-
-Arguments trigger_inl1 {D E} [T].
-
-(** Here's some syntactic sugar with a notation [mrec-fix]. *)
-
-(** Short for endofunctions, used in [mrec_fix] and [rec_fix]. *)
-Local Notation endo T := (T -> T).
-
-Definition mrec_fix {D E : Type -> Type}
-           (ctx : endo (D ~> itree (D +' E)))
-  : D ~> itree E
-  := mrec (ctx trigger_inl1).
-
-Arguments mrec_fix {D E} &.
-
-Notation "'mrec-fix' f d := g" :=
-	(let D := _ in
-	 mrec_fix (D := D) (fun (f : forall T, D T -> _) T (d : D T) => g))
-  (at level 200, f name, d pattern).
-(* No idea what a good level would be. *)
-
-(** *** Simple recursion *)
-
-Inductive callE (A B : Type) : Type -> Type :=
-| Call : A -> callE A B B.
-
-Arguments Call {A B}.
-
-(** Get the [A] contained in a [callE A B]. *)
-Definition unCall {A B T} (e : callE A B T) : A :=
-  match e with
-  | Call a => a
+(** Unfolding of [ext_interp_mrec]. *)
+Definition _interp_mrec2 {R : Type} (ot : itreeF (D +' E) R _) :
+  itree E R :=
+  match ot with
+  | RetF r => Ret r
+  | TauF t => Tau (interp_mrec2 X ctx1 ctx2 t)
+  | VisF _ e k =>
+    match e with
+    | inl1 d =>
+        match mfun1 d with
+        | inl1 d1 => Tau (interp_mrec2 X ctx1 ctx2 (ctx1 d1 >>= k))
+        | inr1 d2 => Tau (interp_mrec2 X ctx1 ctx2 (ctx2 d2 >>= k))                end 
+    | inr1 e => Vis e (fun x => Tau (interp_mrec2 X ctx1 ctx2 (k x)))
+    end
   end.
 
-(** Lift a function on [A] to a morphism on [callE]. *)
-Definition calling {A B} {F : Type -> Type}
-           (f : A -> F B) : callE A B ~> F :=
-  fun _ e =>
-    match e with
-    | Call a => f a
-    end.
+Lemma unfold_interp_mrec2 R (t : itree (D +' E) R) :
+  interp_mrec2 X ctx1 ctx2 t ≅ _interp_mrec2 (observe t).
+Proof.
+  unfold interp_mrec2.
+  rewrite unfold_iter.
+  destruct observe; cbn.
+  - rewrite bind_ret_l; reflexivity.
+  - rewrite bind_ret_l; reflexivity.
+  - destruct e; cbn.
+    + remember (mfun1 d) as dd.
+      destruct dd; cbn.
+      * rewrite bind_ret_l; reflexivity.
+      * rewrite bind_ret_l; reflexivity.  
+    + rewrite bind_vis.
+      pstep; constructor. intros. left.
+      rewrite bind_ret_l; cbn. 
+      eapply eqit_Tau; reflexivity.
+Qed.
 
-(* TODO: This is identical to [callWith] but [rec] finds a universe
-   inconsistency with [calling], and not with [calling'].
-   The inconsistency now pops up later (currently in [Events.Env]) *)
-Definition calling' {A B} {F : Type -> Type}
-           (f : A -> itree F B) : callE A B ~> itree F :=
-  fun _ e =>
-    match e with
-    | Call a => f a
-    end.
+(** [mrec2] is equivalent to [interp (mrecursive2)] *)
+Definition mrecursive2 : (D +' E) ~> itree E := fun _ m =>
+  match m with
+  | inl1 m => mrec2 X ctx1 ctx2 m
+  | inr1 m => ITree.trigger m
+  end.
 
-(* Interpret a single recursive definition. *)
-Definition rec {E : Type -> Type} {A B : Type}
-           (body : A -> itree (callE A B +' E) B) :
-  A -> itree E B :=
-  fun a => mrec (calling' body) (Call a).
+Global Instance eq_itree_mrec2 {R} :
+  Proper (eq_itree eq ==> eq_itree eq)
+    (@interp_mrec2 _ _ _ _ X ctx1 ctx2 R).
+Proof.
+  ginit. gcofix CIH. intros.
+  rewrite !unfold_interp_mrec2.
+  punfold H0. inv H0; try discriminate; pclearbot;
+    simpobs; [| |destruct e]; gstep.
+  - apply reflexivity.
+  - econstructor. eauto with paco.
+  - simpl. remember (mfun1 d) as dd.
+    destruct dd.
+    + econstructor. gbase. eapply CIH. apply eqit_bind; auto; reflexivity.
+    + econstructor. gbase. eapply CIH. apply eqit_bind; auto; reflexivity.
+  - econstructor. gstep; constructor. auto with paco itree.    
+Qed.
 
-Arguments rec {E A B} &.
-
-(** An easy way to construct an event suitable for use with [rec].
-    [call] is an event representing the recursive call.  Since in general, the
-    function might have other events of type [E], the resulting itree has
-    type [(callE A B +' E)].
-*)
-Definition call {E A B} (a:A) : itree (callE A B +' E) B := ITree.trigger (inl1 (Call a)).
-
-(** Here's some syntactic sugar with a notation [mrec-fix]. *)
-
-Definition rec_fix {E : Type -> Type} {A B : Type}
-           (body : endo (A -> itree (callE A B +' E) B))
-  : A -> itree E B
-  := rec (body call).
-
-Arguments rec_fix {E A B} &.
-
-Notation "'rec-fix' f a := g" := (rec_fix (fun f a => g))
-  (at level 200, f name, a pattern).
-(* No idea what a good level would be. *)
+Theorem interp_mrec2_as_interp {T} (c : itree _ T) :
+  interp_mrec2 X ctx1 ctx2 c ≈ interp mrecursive2 c.
+Proof.
+  setoid_rewrite <- interp_mrec2_ok.
+  setoid_rewrite interp_mrec_as_interp.
+  eapply eutt_interp; try reflexivity.
+  intros T0 [a | a]; try reflexivity.
+  setoid_rewrite <- interp_mrec2_ok; reflexivity.  
+Qed.  
+  
+End Facts.
 
 
-*)
+
